\documentclass[conference]{IEEEtran}
\usepackage{babel}
\usepackage[utf8]{vietnam}
\usepackage{mathtools}
\usepackage{graphicx}
\usepackage{graphics}
\usepackage{epstopdf}
\usepackage{amsfonts}
\begin{document}
	\begin{equation*}
	L = L_0e^{-kd} + L_{\infty}(1 - e^{-kd})
	\end{equation*}
	\begin{align*}
	&L = (L_0 - L_\infty)e^{-kd} + L_\infty\\
	&\frac{L - L_\infty}{L_\infty} = \frac{L_0 - L_\infty}{L_\infty}e^{-kd}\\
	&C = C_0e^{-kd}
	\end{align*}
	\begin{equation*}
	d = -\frac{1}{k}\ln{\frac{C}{C_0}}
	\end{equation*}
	\begin{equation*}
	\frac{C}{C_0} \ge 0.05
	\end{equation*}
	\begin{equation*}
	d_{vis} = -\frac{1}{k}\ln{(0.05)} \approx \frac{3}{k}
	\end{equation*}
	\[
	\begin{cases*}	
	 u = u_0 + \alpha\frac{x}{z}\\
	 v = v_0 + \alpha\frac{y}{z} 
	 \end{cases*}
	\]
	\begin{equation*}
	v_h = v_0 - \alpha\tan{\theta}
	\end{equation*}
	\begin{align*}
	L &= (L_0 - L_\infty)e^{-kd} + L_\infty\\
	  &= (L_0 - L_\infty)e^{\frac{-k\lambda}{v - v_h}} + L_\infty
	\end{align*}
	\begin{equation*}
	\frac{dL}{dv} = \frac{k\lambda(L_0 - L_\infty)}{(v - v_h)^2}e^{\frac{-k\lambda}{v - v_h}}
	\end{equation*}
	\begin{equation*}
	\frac{d^2L}{dv^2} = \frac{k\lambda(L_0 - L_\infty)}{(v - v_h)^3}e^{\frac{-k\lambda}{v - v_h}}(\frac{k\lambda}{v - v_h} - 2)
	\end{equation*}
	$\frac{d^2L}{dv^2} = 0$ khi $\frac{k\lambda}{v - v_h} - 2 = 0$\\
	\newline
	$v_i = v_h + \frac{k\lambda}{2}$
	\begin{equation*}
	k = \frac{2(v_i - v_h)}{\lambda} = \frac{2}{d_i} 
	\end{equation*}
	\begin{equation*}
	d_{vis} = \frac{3}{k} = \frac{3\lambda}{2(v_i - v_h)}
	\end{equation*}
\end{document}